src/Parsers/Refinement/SharpenedExpressionPlusParen.v
@@ -1,0 +1,71 @@
+(** Sharpened ADT for an expression grammar with + and () *)
+Require Import Coq.Init.Wf Coq.Arith.Wf_nat.
+Require Import Coq.Lists.List.
+Require Import Coq.Numbers.Natural.Peano.NPeano.
+Require Import Fiat.Parsers.Refinement.Tactics.
+Require Import Fiat.Parsers.Grammars.ExpressionNumPlusParen.
+Require Import Fiat.Computation.Refinements.General.
+Require Import Fiat.Parsers.StringLike.Properties.
+Require Import Fiat.Parsers.StringLike.String.
+Require Import Fiat.Common.
+Require Import Fiat.Common.Equality.
+Require Import Fiat.Common.Wf.
+Require Import Fiat.Parsers.Splitters.RDPList.
+Require Import Fiat.Parsers.BaseTypes.
+Require Import Fiat.Parsers.Refinement.FixedLengthLemmas.
+Require Import Fiat.Parsers.Refinement.DisjointRules.
+Require Import Fiat.Parsers.Refinement.BinOpBrackets.MakeBinOpTable.
+Require Import Fiat.Parsers.Refinement.BinOpBrackets.BinOpRules.
+Require Import Fiat.Parsers.ExtrOcamlParsers. (* for simpl rules for [find_first_char_such_that] *)
+
+Set Implicit Arguments.
+
+Section IndexedImpl.
+  Typeclasses Opaque If_Then_Else.
+
+  (** TODO: generate this automatically? *)
+  Local Instance pbh_plus : paren_balanced_hiding_dataT Ascii.ascii
+    := { is_bin_op := ascii_beq "+"%char;
+         is_open := ascii_beq "("%char;
+         is_close := ascii_beq ")"%char }.
+
+  Lemma ComputationalSplitter'
+  : FullySharpened (string_spec plus_expr_grammar).
+  Proof.
+    start honing parser using indexed representation.
+
+    hone method "splits".
+    {
+      simplify parser splitter.
+      setoid_rewrite refine_binop_table''; [ | apply list_of_next_bin_ops_satisfies_spec | reflexivity.. ].
+      simpl.
+      finish honing parser method.
+    }
+
+    FullySharpenEachMethodWithoutDelegation.
+    extract delegate-free implementation.
+    simpl; higher_order_reflexivityT.
+  Defined.
+
+  Lemma ComputationalSplitter
+  : FullySharpened (string_spec plus_expr_grammar).
+  Proof.
+    let impl := (eval simpl in (projT1 ComputationalSplitter')) in
+    refine (existT _ impl _).
+    abstract (exact (projT2 ComputationalSplitter')).
+  Defined.
+
+End IndexedImpl.
+
+Global Arguments ComputationalSplitter / .
+
+Require Import Fiat.Parsers.ParserFromParserADT.
+Require Import Fiat.Parsers.ExtrOcamlParsers.
+Import Fiat.Parsers.ExtrOcamlParsers.HideProofs.
+
+Time Definition paren_expr_parser (str : String.string) : bool
+  := Eval simpl in has_parse (parser ComputationalSplitter) str.
+
+Print paren_expr_parser.
+
+Recursive Extraction paren_expr_parser.
